Put AES encrypt and decrypt proofs in one file in the tutorial (2nd attempt).

arm/tutorial/aes_encrypt_decrypt.ml
@@ -141,3 +141,121 @@ let AES256_ENCRYPT_CORRECT = prove(
   (* GEN_REWRITE_TAC LAND_CONV [WORD_XOR_SYM] THEN
     REFL_TAC *)
 );;
+
+(******************************************************************************
+  AES-256 decryption proof.
+******************************************************************************)
+
+needs "arm/proofs/utils/aes_decrypt_spec.ml";;
+
+(* The following program performs an AES-256 decryption,
+   with the following differences from encryption (see tutorial/aes_encrypt.ml):
+
+   procedure EQINVCIPHER(in, Nr, dw) is the one used from the standard in order
+   to be able to use the same round keys in the same order as with encrypt.
+
+   The instructions AESD and AESIMC form one AES decryption round:
+   AESD: AESInvSubBytes(AESInvShiftRows(operand1 XOR operand2),   // XOR = AddRoundKey
+   AESIMC: AESInvMixColumns(operand)
+   The last round doesn't use AESIMC, only AESD and XOR.
+*)
+
+let aes256_decrypt_mc = define_assert_from_elf "aes256_decrypt_mc" "arm/tutorial/aes_decrypt.o"
+[
+  0xb940f046;       (* arm_LDR W6 X2 (Immediate_Offset (word 240)) *)
+  0x4cdf7040;       (* arm_LDR Q0 X2 (Postimmediate_Offset (word 16)) *)
+  0x4cdf7041;       (* arm_LDR Q1 X2 (Postimmediate_Offset (word 16)) *)
+  0x4c407026;       (* arm_LDR Q6 X1 No_Offset *)
+  0x510008c6;       (* arm_SUB W6 W6 (rvalue (word 2)) *)
+  0x4e285806;       (* arm_AESD Q6 Q0 *)
+  0x4e2878c6;       (* arm_AESIMC Q6 Q6 *)
+  0x4cdf7840;       (* arm_LDR Q0 X2 (Postimmediate_Offset (word 16)) *)
+  0x710008c6;       (* arm_SUBS W6 W6 (rvalue (word 2)) *)
+  0x4e285826;       (* arm_AESD Q6 Q1 *)
+  0x4e2878c6;       (* arm_AESIMC Q6 Q6 *)
+  0x4cdf7841;       (* arm_LDR Q1 X2 (Postimmediate_Offset (word 16)) *)
+  0x54ffff2c;       (* arm_BGT (word 2097124) *)
+  0x4e285806;       (* arm_AESD Q6 Q0 *)
+  0x4e2878c6;       (* arm_AESIMC Q6 Q6 *)
+  0x4c407840;       (* arm_LDR Q0 X2 No_Offset *)
+  0x4e285826;       (* arm_AESD Q6 Q1 *)
+  0x6e201cc6;       (* arm_EOR_VEC Q6 Q6 Q0 128 *)
+  0x4c007806        (* arm_STR Q6 X0 No_Offset *)
+];;
+
+let AES256_DECRYPT_EXEC = ARM_MK_EXEC_RULE aes256_decrypt_mc;;
+
+let AES256_DECRYPT_CORRECT = prove(
+  `!plaintext ciphertext key ib k0 k1 k2 k3 k4 k5 k6 k7 k8 k9 k10 k11 k12 k13 k14 pc.
+    nonoverlapping (word pc,LENGTH aes256_decrypt_mc) (plaintext,16)
+    ==> ensures arm
+      // precondition
+      (\s. aligned_bytes_loaded s (word pc) aes256_decrypt_mc /\
+           read PC s = word pc /\
+           // uses the C ABI which puts the arguments in their order in registers x0 to x7.
+           // Here only 3 arguments are passed in.
+           C_ARGUMENTS [plaintext; ciphertext; key] s /\
+           read(memory :> bytes128 ciphertext) s = ib /\
+           read(memory :> bytes32 (word_add key (word 240))) s = word 14 /\
+           read(memory :> bytes128 key) s = k0 /\
+           read(memory :> bytes128 (word_add key (word 16))) s = k1 /\
+           read(memory :> bytes128 (word_add key (word 32))) s = k2 /\
+           read(memory :> bytes128 (word_add key (word 48))) s = k3 /\
+           read(memory :> bytes128 (word_add key (word 64))) s = k4 /\
+           read(memory :> bytes128 (word_add key (word 80))) s = k5 /\
+           read(memory :> bytes128 (word_add key (word 96))) s = k6 /\
+           read(memory :> bytes128 (word_add key (word 112))) s = k7 /\
+           read(memory :> bytes128 (word_add key (word 128))) s = k8 /\
+           read(memory :> bytes128 (word_add key (word 144))) s = k9 /\
+           read(memory :> bytes128 (word_add key (word 160))) s = k10 /\
+           read(memory :> bytes128 (word_add key (word 176))) s = k11 /\
+           read(memory :> bytes128 (word_add key (word 192))) s = k12 /\
+           read(memory :> bytes128 (word_add key (word 208))) s = k13 /\
+           read(memory :> bytes128 (word_add key (word 224))) s = k14)
+      // postcondition
+      (\s. read PC s = word (pc + LENGTH aes256_decrypt_mc) /\
+           read (memory :> bytes128 plaintext) s =
+             aes256_decrypt ib [k0; k1; k2; k3; k4; k5; k6; k7; k8; k9; k10; k11; k12; k13; k14]
+        )
+      // Registers (and memory locations) that may change after execution
+      (MAYCHANGE [PC;X6;X2] ,, MAYCHANGE [Q0; Q1; Q6],,
+       MAYCHANGE [memory :> bytes128 plaintext],,
+       MAYCHANGE SOME_FLAGS,, MAYCHANGE [events])`,
+
+  MAP_EVERY X_GEN_TAC
+   [`plaintext:int64`; `ciphertext:int64`; `key:int64`;
+    `ib:int128`; `k0:int128`; `k1:int128`; `k2:int128`;
+    `k3:int128`; `k4:int128`; `k5:int128`; `k6:int128`;
+    `k7:int128`; `k8:int128`; `k9:int128`; `k10:int128`;
+    `k11:int128`; `k12:int128`; `k13:int128`; `k14:int128`; `pc:num`] THEN
+
+  (* Convert C_ARGUMENTS to reading registers x0, x1, x2 and expand SOME_FLAGS *)
+  REWRITE_TAC[C_ARGUMENTS; SOME_FLAGS] THEN
+
+  (* Find the length of the program using a Conversion *)
+  REWRITE_TAC [(REWRITE_CONV [aes256_decrypt_mc] THENC LENGTH_CONV) `LENGTH aes256_decrypt_mc`] THEN
+  DISCH_THEN(REPEAT_TCL CONJUNCTS_THEN ASSUME_TAC) THEN
+
+  (* Start symbolic execution with state 's0' *)
+  ENSURES_INIT_TAC "s0" THEN
+  (* Symbolic execution of all instructions *)
+  ARM_ACCSTEPS_TAC AES256_DECRYPT_EXEC [] (1--59) THEN
+  (* Returned; Finalize symbolic execution. *)
+  ENSURES_FINAL_STATE_TAC THEN
+  (* Use ASM_REWRITE_TAC[] to rewrite the goal using equalities in assumptions. *)
+  ASM_REWRITE_TAC[] THEN
+
+  (* Use the specs to expand defintions *)
+  REWRITE_TAC [aes256_decrypt] THEN
+
+  (* Replace the elements selection, EL, with the selected element
+     from the key round list. *)
+  REWRITE_TAC EL_15_128_CLAUSES THEN
+
+  (* Expand definitions and evaluate `let` terms *)
+  REWRITE_TAC [aes256_decrypt_round] THEN
+  CONV_TAC(TOP_DEPTH_CONV let_CONV) THEN
+  REWRITE_TAC [aesd;aesimc] THEN
+  GEN_REWRITE_TAC LAND_CONV [WORD_XOR_SYM] THEN
+  REFL_TAC
+);;
